proof/invariants/WritePhyEntryPrepare.v
@@ -182,6 +182,54 @@ apply readPresentMapMMUPage with entry;trivial.
 intuition.
 Qed.
 
+Lemma isWellFormedFstShadowTablesAddIndirection nextIndirection indirection idx entry lpred s:
+lookup indirection idx
+      (memory s) beqPage beqIndex = Some (PE entry) ->
+nextIndirection <> indirection -> 
+isWellFormedFstShadow lpred nextIndirection s ->
+isWellFormedFstShadow lpred nextIndirection {|
+currentPartition := currentPartition s;
+memory := add indirection idx
+            (PE
+               {|
+               read := true;
+               write := true;
+               exec := true;
+               present := true;
+               user := true;
+               pa := nextIndirection |}) (memory s) beqPage beqIndex |}.
+Proof.
+intros Hlookup Hdef Hwell.
+unfold isWellFormedFstShadow in *.
+simpl.
+intros.
+destruct Hwell as [(Hl & Hwell)|(Hl & Hwell)];intros.
++ left.
+split;trivial.
+intros.
+generalize (Hwell idx0 ); clear Hwell ; intros (Hi1 & Hi2).
+rewrite <- Hi1.
+rewrite <- Hi2.
+split.
+symmetry.
+apply readPhyEntryMapMMUPage with entry;trivial.
+left;intuition.
+symmetry.
+apply readPresentMapMMUPage with entry;trivial.
+intuition.
++ right.
+
+split;trivial.
+intros.
+generalize (Hwell idx0 ); clear Hwell ; intros (Hi1 & Hi2).
+rewrite <- Hi1.
+rewrite <- Hi2.
+split.
+symmetry.
+apply readVirEntryMapMMUPage  with entry;trivial.
+apply readPDflagMapMMUPage with entry;trivial.
+Qed.
+
 Lemma getIndirectionAddIndirectionCheckVaddrsFalse  vapg l indirection vaToPrepare nextIndirection p pg indMMUToPrepare entry partition  s:
 let s' := {|
       currentPartition := currentPartition s;
@@ -295,14 +343,14 @@ assert( (StateLib.getIndexOfAddr vaToPrepare l) = (StateLib.getIndexOfAddr vapg 
                   present := true;
                   user := true;
                   pa := nextIndirection |}) (memory s) beqPage beqIndex) = Some defaultPage).
-          assert(Hwell':  isWellFormedMMUTables nextIndirection s').
+          { assert(Hwell':  isWellFormedMMUTables nextIndirection s').
           apply isWellFormedMMUTablesAddIndirection with entry;trivial.
           rewrite Hvadsl;trivial.
           unfold isWellFormedMMUTables in Hwell'.
           generalize (Hwell' (StateLib.getIndexOfAddr vapg fstLevel) ) ; clear Hwell'; intros (Hwell'1 & Hwell'2) .
           simpl in *.
           rewrite <- Hvadsl.
-          trivial.
+          trivial. }
           rewrite Hkey in Hread.
           inversion Hread.
           subst.
@@ -4335,11 +4383,9 @@ indMMUToPrepare partition part;trivial.
 rewrite Heq.  split;intros Hgoal;trivial.
 Qed.
 
-Definition or2 idxroot:=
-(idxroot=PDidx \/ idxroot = sh2idx).
 
-Definition or3 idxroot:=
-(idxroot=PDidx \/ idxroot=sh1idx \/ idxroot = sh2idx).
+
+
 
 Lemma checkChildAddIndirectionSamePartPdSh2 indirection idx  vavalue nextIndirection idxroot nbLgen part  e w r entry pd s:
  or2 idxroot ->
@@ -4460,19 +4506,29 @@ assert(Hpdflag: StateLib.readPDflag p (StateLib.getIndexOfAddr vavalue fstLevel)
      trivial.
 Qed.
 
-Lemma checkChildAddIndirectionSamePartSh1 indirection idx  vavalue nextIndirection  nbLgen part  e w r entry sh1 s:
-lookup indirection idx (memory s) beqPage beqIndex = Some (PE entry) ->
+
+Lemma checkChildAddIndirectionSamePartSh1 indirection   vavalue nextIndirection 
+vaToPrepare nbLgen part  e w r entry sh1 l lpred s b:
+lookup indirection  (StateLib.getIndexOfAddr vaToPrepare l) (memory s) beqPage beqIndex = Some (PE entry) ->
 partitionDescriptorEntry s ->
 noDupConfigPagesList s ->
+isPresentNotDefaultIff s ->
+noDupConfigPagesList s ->
+configTablesAreDifferent s ->
 nextEntryIsPP part sh1idx sh1 s ->
 In indirection (getIndirections sh1 s) ->
+indirectionDescription s part indirection sh1idx vaToPrepare l ->
 In part (getPartitions multiplexer s)  ->
 Some nbLgen = StateLib.getNbLevel ->
+StateLib.Level.eqb l fstLevel = false ->
 (forall idx, StateLib.readPhyEntry indirection idx (memory s) = Some defaultPage) ->
- checkChild part nbLgen s vavalue  =
+StateLib.Level.pred l = Some lpred ->
+isWellFormedFstShadow lpred nextIndirection s ->
+ checkChild part nbLgen s vavalue  = b ->
+ (defaultPage =? nextIndirection) = false ->
 checkChild part nbLgen  {|
   currentPartition := currentPartition s;
-  memory := add indirection  idx
+  memory := add indirection   (StateLib.getIndexOfAddr vaToPrepare l)
               (PE
                  {|
                  read := r;
@@ -4480,15 +4536,16 @@ checkChild part nbLgen  {|
                  exec := e;
                  present :=true;
                  user := true;
-                 pa := nextIndirection |}) (memory s) beqPage beqIndex |} vavalue .
+                 pa := nextIndirection |}) (memory s) beqPage beqIndex |} vavalue = b.
 Proof.
 set(s':={|currentPartition:= _ |}) in *.
-intros  Hlookup Hpde Hconfdiff Hpd Hkey Hpart Hnbl Hread.
-unfold checkChild.
+intros  Hlookup Hpde Hconfdiff Hcons1 Hcons2 Hcons3 Hpd Hkey Hroot Hpart Hl Hlevel Hread Hwell1 Hwell2 Hvapg
+Hnextnotdef.
+unfold checkChild in *.
 simpl.
 assert(Hgetsh1 : forall part, getFstShadow part (memory s) =
  getFstShadow part
-    (add indirection  idx
+    (add indirection   (StateLib.getIndexOfAddr vaToPrepare l)
               (PE
                  {|
                  read := r;
@@ -4499,10 +4556,11 @@ assert(Hgetsh1 : forall part, getFstShadow part (memory s) =
                  pa := nextIndirection |}) (memory s) beqPage beqIndex )).
 { intros. symmetry.
   apply getFstShadowMapMMUPage with entry;trivial. }
-rewrite <- Hgetsh1. clear Hgetsh1.
+rewrite <- Hgetsh1. 
+
  unfold noDupConfigPagesList in *.
 generalize(Hconfdiff part Hpart);clear Hconfdiff; intros Hconfdiff.
-unfold getConfigPages in Hconfdiff.
+(* unfold getConfigPages in Hconfdiff.
 apply NoDup_cons_iff in Hconfdiff.
 destruct Hconfdiff as (_ & Hconfdiff).
 unfold getConfigPagesAux in *.
@@ -4518,88 +4576,924 @@ rewrite Hpd1, Hsh11, Hsh2, Hsh3 in Hconfdiff.
 assert(sh1 = sh11).
 apply getSh1NextEntryIsPPEq with part s;trivial.
 subst sh11.
-rewrite Hsh11.
-(*
-case_eq( getIndirection sh1 vavalue nbLgen (nbLevel - 1) s);
-intros * Hind.
-+ case_eq( getIndirection sh1 vavalue nbLgen (nbLevel - 1) s');
-  intros * Hind'.
-  -  case_eq(p =? defaultPage);intros * Hdef.
-    * case_eq(p0 =? defaultPage);intros * Hdef';trivial.
-      (** contradiction *) admit. 
-    * case_eq(p0 =? defaultPage);intros * Hdef';trivial.
-     ++ case_eq(StateLib.readPDflag p (StateLib.getIndexOfAddr vavalue fstLevel) (memory s));intros * Hflag;trivial.
-        case_eq b;intros;subst;trivial.
-           (** contradiction **) admit.
-     ++ 
+rewrite Hsh11. *)
+rewrite nextEntryIsPPgetFstShadow in *.
+rewrite Hpd in *.
+assert(Hnodup : NoDup (getIndirections sh1 s)).
+{ eapply noDupConfigPagesListNoDupGetIndirections with part sh1idx ;trivial.
+right;left;trivial.
+apply nextEntryIsPPgetFstShadow;trivial. }
+unfold indirectionDescription,  initPEntryTablePreconditionToPropagatePrepareProperties in *.
+destruct Hroot as (tableroot & Hpp & Hrootnotdef & Hor).
+ assert(Hpdor: tableroot=sh1).
+ { apply getSh1NextEntryIsPPEq with part s;trivial. }
+  subst tableroot.
+ generalize (Hread (StateLib.getIndexOfAddr vaToPrepare l));clear Hread;intros Hread.  
+destruct Hor as [(Heq & HnbL) | (nbL & stop & HnbL & Hstop & Hindi & Hnotdef & Hstopl)].
+
++ subst indirection;rewrite <- HnbL in *.
+      inversion Hl;subst nbLgen.
+  assert(Hvaddr: StateLib.checkVAddrsEqualityWOOffset nbLevel vaToPrepare vavalue l = true \/
+  StateLib.checkVAddrsEqualityWOOffset nbLevel vaToPrepare vavalue l = false)
+  by (destruct (StateLib.checkVAddrsEqualityWOOffset);[left|right];trivial).
+  destruct Hvaddr as [Hvaddr|Hvaddr].
+  - destruct b.
+    *
+   case_eq(getIndirection sh1 vavalue l (nbLevel - 1) s );[intros tbl Htbl |intros Htbl]; rewrite Htbl in *;
+   try now contradict Hvapg. (** ici il faut montrer que indMMUToPrepare = tbl**)
+
+    case_eq(tbl =? defaultPage);intros Hinddef;rewrite Hinddef in *;try now contradict Hvapg.
+    assert(Hind :  getIndirection sh1 vaToPrepare l (nbLevel - 1) s = Some defaultPage).
+    { apply getIndirectionNbLevelEq with 1; try omega.
+      apply getNbLevelEq in HnbL.
+      subst.
+      inversion Hl;subst.
+      apply nbLevelEq.
+
+      apply levelEqBEqNatFalse0 in Hlevel.
+      omega.
+      simpl.
+      rewrite  Hlevel.
+      rewrite Hread.
+      rewrite <- beq_nat_refl;trivial. }
+      assert(Htrue : getIndirection sh1 vavalue l (nbLevel - 1) s =
+      getIndirection sh1 vaToPrepare l (nbLevel - 1) s).
+      symmetry.
+      apply getIndirectionEq;trivial.
+      destruct l;simpl;omega.
+      rewrite Hind in Htrue.
+      rewrite Htbl in Htrue.
+      inversion Htrue.
+      subst.
+      apply beq_nat_false in Hinddef.
+      omega.
+     * case_eq(getIndirection sh1 vavalue l (nbLevel - 1) s');intros * Htbl;trivial.
+      case_eq(p =? defaultPage);intros * Hp;trivial.
+      admit.
       
- admit. 
+     
+  - assert(Hidxeq: (StateLib.getIndexOfAddr vaToPrepare l) = (StateLib.getIndexOfAddr vavalue l) \/
+ (StateLib.getIndexOfAddr vaToPrepare l) <> (StateLib.getIndexOfAddr vavalue l)) by apply indexDecOrNot.
+  destruct Hidxeq as [Hidxeq |Hidxeq].
+  * rewrite  Hidxeq in Hread.
+    assert(Hind :  getIndirection sh1 vavalue l (nbLevel - 1) s = Some defaultPage).
+    {  apply getIndirectionNbLevelEq with 1; try omega.
+      apply getNbLevelEq in HnbL.
+      subst.
+      inversion Hl;subst.
+      apply nbLevelEq.
+
+      apply levelEqBEqNatFalse0 in Hlevel.
+      omega.
+      simpl.
+      rewrite  Hlevel.
+      rewrite Hread.
+      rewrite <- beq_nat_refl;trivial.
+      
+       } (* 
+    rewrite Hind in Hvapg.
+    assert(Htrue : (defaultPage =? defaultPage )=true).
+    symmetry. apply beq_nat_refl.
+    rewrite Htrue in *.
+    subst b. *)
+     destruct (nbLevel - 1); simpl in *.
+   --  assert(Htru: (sh1 =? defaultPage) = false ).
+        { apply Nat.eqb_neq;trivial.  contradict Hrootnotdef.
+          destruct sh1;destruct defaultPage;simpl in *.
+          subst.
+          f_equal.
+          apply proof_irrelevance. }
+        
+     rewrite Htru in *.
+     rewrite Hidxeq.
+     assert(StateLib.readPDflag sh1 (StateLib.getIndexOfAddr vavalue fstLevel)
+    (add sh1 (StateLib.getIndexOfAddr vavalue l)
+       (PE {| read := r; write := w; exec := e; present := true; user := true; pa := nextIndirection |})
+       (memory s) beqPage beqIndex) = StateLib.readPDflag sh1 (StateLib.getIndexOfAddr vavalue fstLevel) (memory s)
+       ).
+       apply readPDflagMapMMUPage with entry;trivial.
+       rewrite <- Hidxeq.
+       trivial.
+       rewrite H.
+       trivial.
+   -- rewrite Hind in Hvapg.
+      assert(Htrue : (defaultPage =? defaultPage )=true).
+      symmetry. apply beq_nat_refl.
+      rewrite Htrue in *.
+      subst b.
+
+      rewrite Hlevel in *.
+      rewrite Hidxeq.
+
+      assert(Hreadeq:  StateLib.readPhyEntry sh1 (StateLib.getIndexOfAddr vavalue l)
+      (add sh1 (StateLib.getIndexOfAddr vavalue l)
+      (PE {| read := r; write := w; exec := e; present := true; user := true; pa := nextIndirection |})
+      (memory s) beqPage beqIndex) = Some nextIndirection ).
+      {  apply readPhyEntryAddIndirectionSameTable.
+        }
+      rewrite Hreadeq.
+      rewrite Hread in *.
+      assert(Hnext:(defaultPage =? nextIndirection) = false) by trivial.
+      rewrite Hnext.
+      case_eq(StateLib.Level.pred l );intros;trivial.
+           assert(Hpdflag: StateLib.readPDflag nextIndirection (StateLib.getIndexOfAddr vavalue fstLevel)
+      (add sh1 (StateLib.getIndexOfAddr vavalue l)
+      (PE {| read := r; write := w; exec := e; present := true; user := true; pa := nextIndirection |})
+      (memory s) beqPage beqIndex) = StateLib.readPDflag nextIndirection (StateLib.getIndexOfAddr vavalue fstLevel) (memory s)
+      ).
+      apply readPDflagMapMMUPage with entry;trivial.
+             rewrite <- Hidxeq. trivial.
+      destruct n;simpl;trivial.
+      assert(Hnext':(nextIndirection =? defaultPage) = false).
+      { apply beq_nat_false in Hnext .
+     apply Nat.eqb_neq.
+     intuition. }
+      rewrite Hnext'.
+      unfold isWellFormedFstShadow in *.
+       
+             rewrite Hpdflag.
+      move Hwell2 at bottom.      
+      destruct Hwell2 as [(Hlpred &Hwell2)|(Hlpred &Hwell2)].
+      ++ 
+
+      
+       generalize(Hwell2 (StateLib.getIndexOfAddr vavalue fstLevel) ); clear Hwell2; intros (Hwell2 & _).
+       unfold StateLib.readPhyEntry , StateLib.readPDflag in *.
+       case_eq( lookup nextIndirection (StateLib.getIndexOfAddr vavalue fstLevel) (memory s) beqPage beqIndex);intros *
+       Hwell22;rewrite Hwell22 in *;trivial.
+       destruct v;trivial.
+       now contradict Hwell2.
+     ++
+       generalize(Hwell2 (StateLib.getIndexOfAddr vavalue fstLevel) ); clear Hwell2; intros (_ & Hwell2).
+
+rewrite Hwell2;trivial.
+++ case_eq( StateLib.Level.eqb l0 fstLevel);intros.
+**  
+ assert(Hnext':(nextIndirection =? defaultPage) = false).
+      { apply beq_nat_false in Hnext .
+     apply Nat.eqb_neq.
+     intuition. }
+      rewrite Hnext'.
+      rewrite Hpdflag. 
+      move Hwell2 at bottom.      
+      destruct Hwell2 as [(Hlpred &Hwell2)|(Hlpred &Hwell2)].
+
+ 
+
+      
+       generalize(Hwell2 (StateLib.getIndexOfAddr vavalue fstLevel) ); clear Hwell2; intros (Hwell2 & _).
+       unfold StateLib.readPhyEntry , StateLib.readPDflag in *.
+       case_eq( lookup nextIndirection (StateLib.getIndexOfAddr vavalue fstLevel) (memory s) beqPage beqIndex);intros *
+       Hwell22;rewrite Hwell22 in *;trivial.
+       destruct v;trivial.
+       now contradict Hwell2.
+    
+       generalize(Hwell2 (StateLib.getIndexOfAddr vavalue fstLevel) ); clear Hwell2; intros (_ & Hwell2).
+
+rewrite Hwell2;trivial.
+**
+assert(Hup: StateLib.readPhyEntry nextIndirection (StateLib.getIndexOfAddr vavalue l0)
+      (add sh1 (StateLib.getIndexOfAddr vaToPrepare l)
+         (PE {| read := r; write := w; exec := e; present := true; user := true; pa := nextIndirection |})
+         (memory s) beqPage beqIndex)=
+         StateLib.readPhyEntry nextIndirection (StateLib.getIndexOfAddr vavalue l0)
+      
+         (memory s) ).
+         { assert(Hwell':  isWellFormedFstShadow lpred nextIndirection s').
+         
+         unfold s'.
+          apply isWellFormedFstShadowTablesAddIndirection. with entry;trivial.
+          rewrite Hvadsl;trivial.
+          unfold isWellFormedMMUTables in Hwell'.
+          generalize (Hwell' (StateLib.getIndexOfAddr vapg fstLevel) ) ; clear Hwell'; intros (Hwell'1 & Hwell'2) .
+          simpl in *.
+          rewrite <- Hvadsl.
+          trivial. }
+         
+         admit.
+         rewrite Hup.
+         clear Hup.
+          move Hwell2 at bottom.      
+      destruct Hwell2 as [(Hlpred &Hwell2)|(Hlpred &Hwell2)].
+
+ 
+
+      
+       generalize(Hwell2 (StateLib.getIndexOfAddr vavalue l0) ); clear Hwell2; intros (Hwell2 & _).
+       rewrite Hwell2.
+       assert(Hok: (defaultPage =? defaultPage) = true).
+      symmetry. apply beq_nat_refl.
+      
+      rewrite Hok.
+      rewrite Hok;trivial.
+        
+       generalize(Hwell2 (StateLib.getIndexOfAddr vavalue l0) ); clear Hwell2; intros (_ & Hwell2).
+   
+      
+      
+       unfold StateLib.readPhyEntry , StateLib.readPDflag in *.
+       case_eq( lookup nextIndirection (StateLib.getIndexOfAddr vavalue l0) (memory s) beqPage beqIndex);intros *
+       Hwell22;rewrite Hwell22 in *;trivial.
+       destruct v;trivial.
+       now contradict Hwell2.
+  * assert (getIndirection sh1 vavalue l (nbLevel - 1) s = getIndirection sh1 vavalue l (nbLevel - 1) s').
+  { clear Hvapg.  
+ destruct (nbLevel - 1); simpl. trivial.
+ case_eq (StateLib.Level.eqb l fstLevel); intros * Hflst;trivial.
+
+  assert(Hread': StateLib.readPhyEntry sh1 (StateLib.getIndexOfAddr vavalue l)
+        (add sh1 (StateLib.getIndexOfAddr vaToPrepare l)
+               (PE
+                  {|
+                  read := r;
+                  write := w;
+                  exec := e;
+                  present := true;
+                  user := true;
+                  pa := nextIndirection |}) (memory s) beqPage beqIndex)=
+          StateLib.readPhyEntry sh1 (StateLib.getIndexOfAddr vavalue l) (memory s)).
+   {       symmetry. apply readPhyEntryMapMMUPage with entry;trivial.
+          right;trivial.
+          intuition. }
+   rewrite Hread'.
+   case_eq(StateLib.readPhyEntry sh1 (StateLib.getIndexOfAddr vavalue l) (memory s));intros;trivial.        
+   case_eq(defaultPage =? p);intros notdef;trivial.
+   case_eq ( StateLib.Level.pred l);intros * Hlpred;trivial.  
+  apply getIndirectionMapMMUPage11 with entry;trivial.
+  intros.
+ {
+  pose proof indirectionNotInPreviousMMULevelAux.
+  assert(Hor: stop < l \/ stop >= l) by omega.
+  destruct Hor as [Hor | Hor].
+ 
+*
+  generalize(H2 vavalue s (S stop) sh1 l tbl);clear H2;intros H2.
+  replace (S stop - 1) with stop in * by omega.
+ 
+  assert(Hprevious: exists prevtab : page,
+       getIndirection sh1 vavalue l stop s = Some prevtab /\
+       prevtab <> defaultPage /\
+       StateLib.readPhyEntry prevtab (StateLib.getIndexOfAddr vavalue (CLevel (l - stop))) (memory s) = Some tbl).
+ { apply H2;clear H2;try omega.
+ intuition.
+  simpl.
+  rewrite Hlevel.
+  rewrite H.
+  rewrite notdef.
+  rewrite Hlpred;trivial.
+  trivial. }
+  destruct Hprevious as (prevtab & Hprevtable & Hprevnotnull & Hreadprev).
+assert(~ In tbl (getIndirectionsAux sh1 s (stop + 1))).
+{ apply getIndirectionInGetIndirections2 with prevtab vavalue l;
+simpl; subst;
+trivial.
+destruct l;simpl in *.
+omega.
+replace(stop + 1 - 1) with stop in * by omega.
+trivial.
+replace(stop + 1 - 1) with stop in * by omega.
+trivial.
+
+unfold getIndirections in Hnodup.
+apply noDupPreviousMMULevels with nbLevel.
+trivial.
+destruct l.
+simpl in *.
+omega.
+assert((defaultPage =? tbl) = false) as Hnotdef  by trivial.
+apply beq_nat_false in Hnotdef.
+unfold not;intros;subst.
+now contradict Hnotdef.
+destruct l.
+simpl in *.
+omega.
+}
+assert( In sh1 (getIndirectionsAux sh1 s (stop + 1))).
+{ replace  (stop + 1) with (S stop) by omega.
+  simpl.
+  left;trivial. }
+unfold not;intros.
+subst.
+now contradict H4.
+* assert(getIndirection p vavalue l0 (nbLevel -2) s = Some tbl ).
+unfold StateLib.Level.pred in *.
+case_eq( gt_dec l 0);intros * Hl0;rewrite Hl0 in *; try now contradict Hlpred.
+inversion Hlpred.
+apply getIndirectionStopLevelGT2 with stop;simpl in *;
+subst;trivial.
+omega.
+assert(Hlx: l = CLevel (nbLevel - 1)).
+apply getNbLevelEq;trivial.
+pose proof nbLevelEq as Heq.
+rewrite <- Hlx in Heq.
+rewrite <- Heq.
+omega.
+  generalize(H2 vavalue s (nbLevel - 1) sh1 l tbl);clear H2;intros H2.
+(*   replace (S stop - 1) with stop in * by omega.
+   *)
+   assert(Hlx: l = CLevel (nbLevel - 1)).
+apply getNbLevelEq;trivial.
+pose proof nbLevelEq as Heq.
+rewrite <- Hlx in Heq.
+
+pose proof nbLevelNotZero as nblnot0.
+assert(l > 0).
+apply levelEqBEqNatFalse0;trivial.
+  assert(Hprevious: exists prevtab : page,
+       getIndirection sh1 vavalue l (nbLevel - 1 -1) s = Some prevtab /\
+       prevtab <> defaultPage /\
+       StateLib.readPhyEntry prevtab (StateLib.getIndexOfAddr vavalue (CLevel (l - (nbLevel - 1 - 1)))) (memory s) = Some tbl).
+ { apply H2;clear H2;try omega.
+intuition.
 
 
 
+replace (nbLevel - 1) with (nbLevel - 2 + 1) by omega.
+clear H0.
+
+replace (nbLevel - 2 + 1) with (S (nbLevel - 2)) by omega.
+simpl.
+rewrite Hlevel.
+rewrite H.
+rewrite notdef.
+rewrite Hlpred;trivial.
+trivial. }
+
+ destruct Hprevious as (prevtab & Hprevtable & Hprevnotnull & Hreadprev).
+assert(~ In tbl (getIndirectionsAux sh1 s ((nbLevel - 2) + 1))).
+{ apply getIndirectionInGetIndirections2 with prevtab vavalue l;
+simpl; subst;
+trivial.
+
+replace (nbLevel - 1) with (nbLevel - 2 + 1) by omega.
+clear H0.
+
+omega.
+replace(nbLevel - 2 + 1 - 1) with  (nbLevel - 1 - 1) in * by omega.
+trivial.
+
+replace(nbLevel - 2 + 1 - 1) with  (nbLevel - 1 - 1) in * by omega.
+trivial.
+replace(nbLevel - 2 + 1 + 1) with  (nbLevel )  by omega.
+unfold getIndirections in Hnodup.
+trivial.
+assert((defaultPage =? tbl) = false) as Hnotdef  by trivial.
+apply beq_nat_false in Hnotdef.
+unfold not;intros;subst.
+now contradict Hnotdef.
+replace(nbLevel - 2 + 1) with  (nbLevel - 1 ) in * by omega.
+omega.
+}
+assert( In sh1 (getIndirectionsAux sh1 s (nbLevel - 2 + 1))) .
+{ replace (nbLevel - 2 + 1) with (S(nbLevel -2)) by omega.
+  simpl.
+  left;trivial. }
+unfold not;intros.
+subst.
+now contradict H4. }
+*
 
 
 
+   apply beq_nat_false in notdef.
+   intuition.
+   subst. now contradict notdef.
+   }
+   rewrite <- H.
+    case_eq( getIndirection sh1 vavalue l (nbLevel - 1) s);intros * Htbl;trivial;rewrite Htbl in *.
+case_eq( p =? defaultPage); intros * Hp;rewrite Hp in *;trivial.
+assert( sh1 <>p).
+ assert(Hlx: l = CLevel (nbLevel - 1)).
+apply getNbLevelEq;trivial.
+pose proof nbLevelEq as Heq.
+rewrite <- Hlx in Heq.
+assert(Ll: l> 0).
+apply levelEqBEqNatFalse0;trivial.
 
-assert(Hind : getIndirection sh1 vavalue nbLgen (nbLevel - 1) s  =
-getIndirection sh1 vavalue nbLgen (nbLevel - 1) s' ).
-{ apply getIndirectionMapMMUPage11 with entry
+assert(Hin:~ In p (getIndirectionsAux sh1 s (nbLevel - 1))).
+{ 
+
+
+ apply indirectionNotInPreviousMMULevel' with (StateLib.getIndexOfAddr vavalue fstLevel)
+ 
+ vavalue part l sh1idx;trivial.
+ right;left;trivial.
+ 
+ symmetry;trivial.
+ apply beq_nat_false in Hp.
+ apply Nat.eqb_neq.
+ intuition.
+ subst;trivial.
+ rewrite Heq;trivial. }
+
+
+ 
+ assert( In sh1 (getIndirectionsAux sh1 s (nbLevel - 1))) .
+ 
+ subst.
+ destruct (nbLevel - 1);simpl.
+ subst.
+ omega.
+ left;trivial.
+ 
+
+unfold not;intros.
+subst.
+now contradict Hin.
+assert(StateLib.readPDflag p (StateLib.getIndexOfAddr vavalue fstLevel) (memory s') =
+StateLib.readPDflag p (StateLib.getIndexOfAddr vavalue fstLevel) (memory s)).
+apply readPDflagMapMMUPage with entry;trivial.
+simpl in H1.
+rewrite  H1;trivial.
+trivial.
++ rewrite <- HnbL in *.
+inversion Hl;subst nbLgen.
+assert (Hstp: stop + 1 <= nbL).
+{ subst. assert((nbL - stop) > 0).
+apply levelEqBEqNatFalse0 in Hlevel ;trivial.
+unfold CLevel in Hlevel.
+case_eq(lt_dec (nbL - stop) nbLevel);intros * Hlt;rewrite Hlt in *.
+simpl in *;trivial.
+destruct nbL;simpl in *.
+omega.
+
+omega. }
+ assert(Hvaddr: StateLib.checkVAddrsEqualityWOOffset (stop+1) vaToPrepare vavalue nbL = true \/
+  StateLib.checkVAddrsEqualityWOOffset (stop+1) vaToPrepare vavalue nbL = false)
+  by (destruct (StateLib.checkVAddrsEqualityWOOffset);[left|right];trivial).
+  destruct Hvaddr as [Hvaddr|Hvaddr].
+  -
+  assert(Hinstop1: getIndirection sh1 vaToPrepare nbL (stop+1) s = Some defaultPage).
+{  
+   (** ici il faut montrer que indMMUToPrepare = tbl**)
+pose proof getIndirectionEqStop as Hindeq.
+assert( getIndirection sh1 vavalue nbL stop s = Some indirection).
+rewrite <- Hindi.
+symmetry.
+apply Hindeq;trivial.
+subst.
+apply checkVAddrsEqualityWOOffsetTrueLe with (stop+1);trivial.
+  omega.
+apply getIndirectionProp' with (StateLib.getIndexOfAddr vaToPrepare (CLevel (nbL - stop))) indirection entry;
+subst;trivial.
+unfold 
+ isEntryPage, StateLib.readPhyEntry in *.
+ destruct ( lookup indirection (StateLib.getIndexOfAddr vaToPrepare (CLevel (nbL - stop))) (memory s) beqPage beqIndex );simpl in *;trivial;
+ try now contradict Hread.
+ destruct v;try now contradict Hread.
+ inversion Hread;trivial.
+
+}
+
+assert(HindeqStop: getIndirection sh1 vaToPrepare nbL (stop + 1) s=
+getIndirection sh1 vavalue nbL (stop + 1) s).
+{
+apply getIndirectionEqStop;subst;trivial. }
+assert(Hdef: getIndirection sh1 vavalue nbL (nbLevel - 1) s = Some defaultPage).
+{ apply getIndirectionNbLevelEq with (stop+1);trivial.
+  omega.
+  apply getNbLevelEq in HnbL.
+  subst.
+  apply nbLevelEq.
+  rewrite HindeqStop in Hinstop1;trivial. }
+
+
+rewrite Hdef in *.
+assert(Htru: (defaultPage =? defaultPage) = true).
+symmetry.
+apply beq_nat_refl.
+rewrite Htru in *.
+destruct b;try now contradict Hvapg.
+
+case_eq(  getIndirection sh1 vavalue nbL (nbLevel - 1) s');intros * Hi;trivial.
+case_eq(p =? defaultPage);intros * Hi2;trivial.
+admit.
+(* now contradict Hread. *)
+
+- (* destruct  b.
+admit. 
+case_eq(getIndirection sh1 vavalue nbL (nbLevel - 1) s);intros * Hind;rewrite Hind in *;try now contradict Hmap.
+admit.
+case_eq(p =? defaultPage);intros * Hnotdef';rewrite Hnotdef' in *;try now contradict Hmap.
+(* case_eq( getIndirection pd vavalue nbL (nbLevel - 1) s');intros * Hind'. *)
+ *)
+assert(Heq: getIndirection sh1 vavalue nbL (nbLevel - 1) s =
+            getIndirection sh1 vavalue nbL (nbLevel - 1) s').
+{  assert(Horlst: (StateLib.getIndexOfAddr vaToPrepare l) = (StateLib.getIndexOfAddr vavalue l) \/  
+(StateLib.getIndexOfAddr vaToPrepare l) <> (StateLib.getIndexOfAddr vavalue l) ) by apply indexDecOrNot.
+destruct Horlst as [Horlst| Horlst].
++
+
+
+ assert( Hnewvaddr: checkVAddrsEqualityWOOffset (stop ) vaToPrepare vavalue nbL = false ).
+{ apply checkVAddrsEqualityWOOffsetFalseS;trivial.
+
+ subst;trivial. }
+apply getIndirectionMapMMUPage11 with entry
 ;trivial.
 intros * Hi1 Hi2.
-apply NoDupSplitInclIff in Hconfdiff.
-destruct Hconfdiff as (Hconfigdiff1 & Hconfdiff).
-unfold disjoint in *.
-destruct Hor as [Hor|Hor];subst.
-+  assert(pd = pd1).
-apply getPdNextEntryIsPPEq with part s;trivial.
-subst pd1. 
-apply Hconfdiff in Hkey.
-clear Hconfdiff.
-rewrite in_app_iff in Hkey.
-apply not_or_and in Hkey.
-destruct Hkey as (Hkey & _).
-assert (Hkey2: In tbl (getIndirections sh1 s)).
-apply getIndirectionInGetIndirections with vavalue nbLgen stop;trivial.
-apply nbLevelNotZero.
-apply beq_nat_falseNot;trivial.
-apply getNbLevelLe;trivial.
-unfold not;intros;subst;try now contradict Hkey2.
-+  assert(pd = sh2).
-apply getSh2NextEntryIsPPEq with part s;trivial.
-subst pd.
-destruct Hconfigdiff1 as (Hconfigdiff1 & Hconfigdiff2).
-apply NoDupSplitInclIff in Hconfigdiff2.
- destruct Hconfigdiff2 as ( _ & Hconfigdiff2).
-unfold disjoint in *.
+assert(Hor : stop0 < stop \/ stop0=stop \/ stop0 > stop) by omega.
+destruct Hor as [Hor | [Hor | Hor]].
+- assert(Hinind: In tbl (getIndirectionsAux sh1  s (stop0+1))).
+{ apply getIndirectionInGetIndirections1 with vavalue nbL;trivial.
+destruct nbL;simpl in *.
+omega.
+apply beq_nat_false in Hi2.
+unfold not;intros;subst;now contradict Hi2.
+ }
+assert(Hnotinind: ~ In indirection (getIndirectionsAux sh1 s (stop))).
+assert(Hex: stop + 1 <= nbLevel).
+destruct nbL;simpl in *.
+omega.
+   
 
-assert (Hkey2: In tbl (getIndirections sh1 s)).
-apply getIndirectionInGetIndirections with vavalue nbLgen stop;trivial.
-apply nbLevelNotZero.
-apply beq_nat_falseNot;trivial.
-apply getNbLevelLe;trivial.
-unfold not;intros;subst;try now contradict Hkey2.
+apply getIndirectionInGetIndirections2' with vaToPrepare nbL;trivial.
+unfold getIndirections in *.
+apply noDupPreviousMMULevels with nbLevel ;trivial.
+omega.
+pose proof inclGetIndirectionsAuxLe as Hproof.
+contradict Hnotinind.
+unfold incl in Hproof.
+apply Hproof with (stop0+1).
+omega.
+subst;trivial.
+-
 
-apply Hconfigdiff2 in Hkey2.
-rewrite in_app_iff in Hkey2.
-apply not_or_and in Hkey2.
-destruct Hkey2 as (Hkey2 & _).
-now contradict Hkey2.
-  }
-  rewrite <- Hind.  
-case_eq(getIndirection sh1 vavalue nbLgen (nbLevel - 1) s);intros * Hp;rewrite Hp in *.
- case_eq( p =? defaultPage);intros * Hdef;trivial.
-assert(Hpdflag: StateLib.readPDflag p (StateLib.getIndexOfAddr vavalue fstLevel) (memory s) =
- StateLib.readPDflag p (StateLib.getIndexOfAddr vavalue fstLevel)
-    (add indirection idx
-       (PE
-          {| read := r; write := w; exec := e; present := true; user := true; pa := nextIndirection |})
-       (memory s) beqPage beqIndex)).
-       symmetry.
-       apply readPDflagMapMMUPage with entry;trivial.
-     rewrite Hpdflag;trivial.
-     trivial.
-     trivial.
-Qed. *)
+subst.
+assert(Hor: stop=0 \/ stop > 0) by omega.
+destruct Hor as [Hor | Hor].
+* subst. simpl in *.
+case_eq( StateLib.Level.eqb nbL fstLevel);intros * Hlvl;rewrite Hlvl in *.
+rewrite CLevelIdentity' in Hlevel.
+rewrite  Hlevel in Hlvl.
+now contradict Hlvl.
+ now contradict Hvaddr.
+* assert(Hrn: S (stop-1) = stop) by omega.
+  apply pageTablesAreDifferentMiddle with (stop-1) s nbLevel sh1 sh1 nbL  vavalue vaToPrepare
+ stop;trivial;try rewrite Hrn;trivial.
+ rewrite checkVAddrsEqualityWOOffsetPermut';trivial.
+ left;trivial.
+ split;trivial.
+ apply getNbLevelEq;trivial.
+apply beq_nat_false in Hi2.
+unfold not;intros;subst;now contradict Hi2.
+-
+assert(Hx: nbLevel - 1 = nbL).
+{
+apply getNbLevelEq in HnbL.
+subst.
+rewrite <- nbLevelEq;trivial. }
+
+assert(Hornbl: stop0>= nbLevel-1 \/ stop0 < nbLevel -1) by omega.
+destruct Hornbl as [Hornbl | Hornbl].
+
+*
+
+  assert(Hinind: In indirection (getIndirectionsAux sh1  s (stop+1))).
+{ apply getIndirectionInGetIndirections1 with vaToPrepare nbL;trivial.
+omega.
+ }
+assert(Hex: stop + 1 <= nbLevel) by omega.
+
+assert(Hnotinind: ~ In tbl (getIndirectionsAux sh1 s (stop+1))).
+{
+
+ 
+ 
+apply getIndirectionInGetIndirections2n with (nbLevel -1) vavalue nbL;trivial;try omega.
+apply getIndirectionStopLevelGe with stop0;trivial.
+omega.
+
+unfold getIndirections in *.
+apply noDupPreviousMMULevels with nbLevel ;trivial.
+omega.
+apply beq_nat_false in Hi2.
+unfold not;intros;subst;now contradict Hi2. }
+
+unfold not;intros;subst;now contradict Hnotinind.
+*   assert(Hinind: In indirection (getIndirectionsAux sh1  s (stop+1))).
+{ apply getIndirectionInGetIndirections1 with vaToPrepare nbL;trivial.
+omega.
+ }
+assert(Hex: stop + 1 <= nbLevel) by omega.
+
+assert(Hnotinind: ~ In tbl (getIndirectionsAux sh1 s (stop+1))).
+{
+
+ 
+apply getIndirectionInGetIndirections2n with stop0 vavalue nbL;trivial;try omega.
+unfold getIndirections in *.
+apply noDupPreviousMMULevels with nbLevel ;trivial.
+omega.
+apply beq_nat_false in Hi2.
+unfold not;intros;subst;now contradict Hi2. }
+
+unfold not;intros;subst;now contradict Hnotinind.
++ assert(checkVAddrsEqualityWOOffset stop vaToPrepare vavalue nbL = true \/
+checkVAddrsEqualityWOOffset stop vaToPrepare vavalue nbL = false) .
+{ destruct (checkVAddrsEqualityWOOffset stop vaToPrepare vavalue nbL).
+  left;trivial.
+  right;trivial. }
+destruct H.
+**  assert(Hinstop1: getIndirection sh1 vaToPrepare nbL (stop+1) s = Some defaultPage).
+{  
+   (** ici il faut montrer que indMMUToPrepare = tbl**)
+pose proof getIndirectionEqStop as Hindeq.
+assert( getIndirection sh1 vavalue nbL stop s = Some indirection).
+rewrite <- Hindi.
+symmetry.
+apply Hindeq;trivial.
+subst.
+apply getIndirectionProp' with (StateLib.getIndexOfAddr vaToPrepare (CLevel (nbL - stop))) indirection entry;
+subst;trivial.
+unfold 
+ isEntryPage, StateLib.readPhyEntry in *.
+ destruct ( lookup indirection (StateLib.getIndexOfAddr vaToPrepare (CLevel (nbL - stop))) (memory s) beqPage beqIndex );simpl in *;trivial;
+ try now contradict Hread.
+ destruct v; try now contradict Hread.
+ inversion Hread;trivial.
+}
+assert(HindeqStop: getIndirection sh1 vaToPrepare nbL stop s=
+getIndirection sh1 vavalue nbL stop  s).
+
+apply getIndirectionEqStop;subst;trivial.
+(* apply beq_nat_true in Hdefcurind. *)
+
+apply getIndirectionMapMMUPage11' with entry
+;trivial.
+intros * Hi1 Hi2.
+assert(Hor : stop0 < stop \/ stop0=stop \/ stop0 > stop) by omega.
+{ destruct Hor as [Hor | [Hor | Hor]].
+- assert(Hinind: In tbl (getIndirectionsAux sh1  s (stop0+1))).
+{ apply getIndirectionInGetIndirections1 with vavalue nbL;trivial.
+destruct nbL;simpl in *.
+omega.
+apply beq_nat_false in Hi2.
+unfold not;intros;subst;now contradict Hi2.
+ }
+assert(Hnotinind: ~ In indirection (getIndirectionsAux sh1 s (stop))).
+{ assert(Hex: stop + 1 <= nbLevel).
+destruct nbL;simpl in *.
+omega.
+   
+
+apply getIndirectionInGetIndirections2' with vaToPrepare nbL;trivial.
+unfold getIndirections in *.
+apply noDupPreviousMMULevels with nbLevel ;trivial.
+omega.
+ }
+
+pose proof inclGetIndirectionsAuxLe as Hproof.
+left.
+contradict Hnotinind.
+unfold incl in Hproof.
+apply Hproof with (stop0+1).
+omega.
+subst;trivial.
+-
+right.  
+
+subst.
+intuition.
+rewrite Hindi in HindeqStop.
+rewrite Hi1 in HindeqStop.
+inversion HindeqStop;subst;trivial. 
+-
+assert(Hx: nbLevel - 1 = nbL).
+{
+apply getNbLevelEq in HnbL.
+subst.
+rewrite <- nbLevelEq;trivial. }
+
+assert(Hornbl: stop0>= nbLevel-1 \/ stop0 < nbLevel -1) by omega.
+destruct Hornbl as [Hornbl | Hornbl].
+
+*
+
+  assert(Hinind: In indirection (getIndirectionsAux sh1  s (stop+1))).
+{ apply getIndirectionInGetIndirections1 with vaToPrepare nbL;trivial.
+omega.
+ }
+assert(Hex: stop + 1 <= nbLevel) by omega.
+
+assert(Hnotinind: ~ In tbl (getIndirectionsAux sh1 s (stop+1))).
+{
+
+ 
+ 
+apply getIndirectionInGetIndirections2n with (nbLevel -1) vavalue nbL;trivial;try omega.
+apply getIndirectionStopLevelGe with stop0;trivial.
+omega.
+
+unfold getIndirections in *.
+apply noDupPreviousMMULevels with nbLevel ;trivial.
+omega.
+apply beq_nat_false in Hi2.
+unfold not;intros;subst;now contradict Hi2. }left.
+
+unfold not;intros;subst;now contradict Hnotinind.
+*   assert(Hinind: In indirection (getIndirectionsAux sh1  s (stop+1))).
+{ apply getIndirectionInGetIndirections1 with vaToPrepare nbL;trivial.
+omega.
+ }
+assert(Hex: stop + 1 <= nbLevel) by omega.
+
+assert(Hnotinind: ~ In tbl (getIndirectionsAux sh1 s (stop+1))).
+{
+
+ 
+apply getIndirectionInGetIndirections2n with stop0 vavalue nbL;trivial;try omega.
+unfold getIndirections in *.
+apply noDupPreviousMMULevels with nbLevel ;trivial.
+omega.
+apply beq_nat_false in Hi2.
+unfold not;intros;subst;now contradict Hi2. }
+left.
+
+unfold not;intros;subst;now contradict Hnotinind.
+ }
+**
+apply getIndirectionMapMMUPage11 with entry
+;trivial.
+intros * Hi1 Hi2.
+assert(Hor : stop0 < stop \/ stop0=stop \/ stop0 > stop) by omega.
+{ destruct Hor as [Hor | [Hor | Hor]].
+- assert(Hinind: In tbl (getIndirectionsAux sh1  s (stop0+1))).
+{ apply getIndirectionInGetIndirections1 with vavalue nbL;trivial.
+destruct nbL;simpl in *.
+omega.
+apply beq_nat_false in Hi2.
+unfold not;intros;subst;now contradict Hi2.
+ }
+assert(Hnotinind: ~ In indirection (getIndirectionsAux sh1 s (stop))).
+assert(Hex: stop + 1 <= nbLevel).
+destruct nbL;simpl in *.
+omega.
+   
+
+apply getIndirectionInGetIndirections2' with vaToPrepare nbL;trivial.
+unfold getIndirections in *.
+apply noDupPreviousMMULevels with nbLevel ;trivial.
+omega.
+pose proof inclGetIndirectionsAuxLe as Hproof.
+contradict Hnotinind.
+unfold incl in Hproof.
+apply Hproof with (stop0+1).
+omega.
+subst;trivial.
+-
+
+subst.
+assert(Hor: stop=0 \/ stop > 0) by omega.
+destruct Hor as [Hor | Hor].
+* subst. simpl in *.
+inversion Hi1;subst.
+
+inversion Hindi;subst.
+now contradict H.
+* assert(Hrn: S (stop-1) = stop) by omega.
+  apply pageTablesAreDifferentMiddle with (stop-1) s nbLevel sh1 sh1 nbL  vavalue vaToPrepare
+ stop;trivial;try rewrite Hrn;trivial.
+ rewrite checkVAddrsEqualityWOOffsetPermut';trivial.
+ left;trivial.
+ split;trivial.
+ apply getNbLevelEq;trivial.
+apply beq_nat_false in Hi2.
+unfold not;intros;subst;now contradict Hi2.
+
+-
+assert(Hx: nbLevel - 1 = nbL).
+{
+apply getNbLevelEq in HnbL.
+subst.
+rewrite <- nbLevelEq;trivial. }
+
+assert(Hornbl: stop0>= nbLevel-1 \/ stop0 < nbLevel -1) by omega.
+destruct Hornbl as [Hornbl | Hornbl].
+
+*
+
+  assert(Hinind: In indirection (getIndirectionsAux sh1  s (stop+1))).
+{ apply getIndirectionInGetIndirections1 with vaToPrepare nbL;trivial.
+omega.
+ }
+assert(Hex: stop + 1 <= nbLevel) by omega.
+
+assert(Hnotinind: ~ In tbl (getIndirectionsAux sh1 s (stop+1))).
+{
+
+ 
+ 
+apply getIndirectionInGetIndirections2n with (nbLevel -1) vavalue nbL;trivial;try omega.
+apply getIndirectionStopLevelGe with stop0;trivial.
+omega.
+
+unfold getIndirections in *.
+apply noDupPreviousMMULevels with nbLevel ;trivial.
+omega.
+apply beq_nat_false in Hi2.
+unfold not;intros;subst;now contradict Hi2. }
+
+unfold not;intros;subst;now contradict Hnotinind.
+*   assert(Hinind: In indirection (getIndirectionsAux sh1  s (stop+1))).
+{ apply getIndirectionInGetIndirections1 with vaToPrepare nbL;trivial.
+omega.
+ }
+assert(Hex: stop + 1 <= nbLevel) by omega.
+
+assert(Hnotinind: ~ In tbl (getIndirectionsAux sh1 s (stop+1))).
+{
+
+ 
+apply getIndirectionInGetIndirections2n with stop0 vavalue nbL;trivial;try omega.
+unfold getIndirections in *.
+apply noDupPreviousMMULevels with nbLevel ;trivial.
+omega.
+apply beq_nat_false in Hi2.
+unfold not;intros;subst;now contradict Hi2. }
+
+unfold not;intros;subst;now contradict Hnotinind.
+ } }
+ 
+ rewrite <- Heq.
+ destruct  b.
+*  
+case_eq(getIndirection sh1 vavalue nbL (nbLevel - 1) s);intros * Hind;
+rewrite Hind in *;try now contradict Hvapg.
+case_eq(p =? defaultPage);intros * Hnotdef';rewrite Hnotdef' in *;try now contradict Hvapg.
+
+(* case_eq( getIndirection pd vavalue nbL (nbLevel - 1) s');intros * Hind'. *)
+
+ 
+ (*
+ 
+ 
+ rewrite Hind.
+ rewrite Hnotdef'.
+ trivial.
+ assert(Hkeyx: p <> indirection \/ StateLib.getIndexOfAddr vavalue fstLevel <> StateLib.getIndexOfAddr vaToPrepare l).
+{    subst.
+    assert(Horx: stop = nbL \/ stop <> nbL) by omega.
+    destruct Horx as [Horx | Horx].
+    subst.
+    replace (nbL - nbL) with 0 in Hlevel.
+    unfold fstLevel in Hlevel.
+    unfold StateLib.Level.eqb in Hlevel.
+    rewrite <- beq_nat_refl in Hlevel.
+    now contradict Hlevel.
+    omega.
+    assert(Hx: nbLevel - 1 = nbL).
+{
+apply getNbLevelEq in HnbL.
+subst.
+rewrite <- nbLevelEq;trivial. }
+ assert(~In p (getIndirectionsAux sh1 s (stop+1))).
+{
+pose proof nbLevelNotZero as HnbL0.
+ 
+apply getIndirectionInGetIndirections2n with (nbLevel - 1) vavalue nbL;trivial;try omega.
+replace (nbLevel - 1 + 1) with nbLevel by omega.
+unfold getIndirections in *.
+trivial.
+apply beq_nat_false in Hnotdef'.
+unfold not;intros;subst;now contradict Hnotdef'. }
+assert(In indirection (getIndirectionsAux sh1 s (stop+1))).
+{ apply getIndirectionInGetIndirections1 with vaToPrepare nbL;trivial.
+omega.
+ }
+ left.
+ unfold not;intros;subst;now contradict H0.
+ }
+ *)
+ 
+ assert(Hpres: StateLib.readPDflag p (StateLib.getIndexOfAddr vavalue fstLevel) (memory s)=
+ StateLib.readPDflag p (StateLib.getIndexOfAddr vavalue fstLevel) (memory s')).
+ { symmetry. apply readPDflagMapMMUPage with entry;trivial. }
+simpl in *.
+
+ rewrite <- Hpres;trivial.
+ *
+
+
+
+case_eq(getIndirection sh1 vavalue nbL (nbLevel - 1) s);intros * Hind;
+rewrite Hind in *;trivial.
+case_eq(p =? defaultPage);intros * Hnotdef';rewrite Hnotdef' in *;trivial.
+
+ assert(Hpres: StateLib.readPDflag p (StateLib.getIndexOfAddr vavalue fstLevel) (memory s)=
+ StateLib.readPDflag p (StateLib.getIndexOfAddr vavalue fstLevel) (memory s')).
+ { symmetry. apply readPDflagMapMMUPage with entry;trivial. }
+simpl in *.
+
+ rewrite <- Hpres;trivial.
+
+
+
+
+
+
+
+
 Admitted.
 
 Lemma checkChildAddIndirection indirection idx  vavalue nextIndirection idxroot nbLgen part  e w r entry pd b s:
@@ -4614,7 +5508,7 @@ In part (getPartitions multiplexer s)  ->
 Some nbLgen = StateLib.getNbLevel ->
 forall partx,
 In partx (getPartitions multiplexer s) ->
- checkChild partx nbLgen s vavalue  = b <->
+ checkChild partx nbLgen s vavalue  = b ->
 checkChild partx nbLgen  {|
   currentPartition := currentPartition s;
   memory := add indirection  idx
@@ -4628,22 +5522,18 @@ checkChild partx nbLgen  {|
                  pa := nextIndirection |}) (memory s) beqPage beqIndex |} vavalue = b.
 Proof.
 set(s':={|currentPartition:= _ |}) in *.
-intros Hor3 Hlookup Hpde Hconfdiff Hdisjoint Hpd Hkey Hpart Hnbl partx Hpartx.
+intros Hor3 Hlookup Hpde Hconfdiff Hdisjoint Hpd Hkey Hpart Hnbl partx Hpartx Hgoal.
 
 assert(Hor: partx = part \/ partx <> part) by apply pageDecOrNot.
 destruct Hor as [Hor|Hor];subst.
 + destruct Hor3 as [Hor3 | [Hor3|Hor]];subst.
-  - assert(Heq: checkChild part nbLgen s vavalue = checkChild part nbLgen s' vavalue). 
+  - symmetry.
   apply checkChildAddIndirectionSamePartPdSh2 with PDidx entry pd ;trivial.
   unfold or2;left;trivial.
-  rewrite Heq.
-  split;trivial.
   - admit. (* checkChildAddIndirectionSamePartSh1 *)
-  - assert(Heq: checkChild part nbLgen s vavalue = checkChild part nbLgen s' vavalue). 
+  - symmetry.
     apply checkChildAddIndirectionSamePartPdSh2 with sh2idx entry pd ;trivial.
   unfold or2;right;trivial.
-  rewrite Heq.
-  split;trivial.
 + unfold checkChild.
   assert(Hgetsh1 : forall part, getFstShadow part (memory s) =
     getFstShadow part
@@ -4697,10 +5587,10 @@ subst;trivial.
 apply sh1PartNotNull with partx s;trivial.
 apply nextEntryIsPPgetFstShadow;trivial. }
 rewrite <- Hindeq.
-case_eq(getIndirection p vavalue nbLgen (nbLevel - 1) s);intros * Hp;rewrite Hp in *;
-[| split;intros;trivial].
+case_eq(getIndirection p vavalue nbLgen (nbLevel - 1) s);intros * Hp;rewrite Hp in *; trivial.
+(*[| split;intros;trivial]. *)
  case_eq( p0 =? defaultPage);intros * Hdef;trivial.
-       split;intros;trivial.
+     (*   split;intros;trivial. *)
 assert(Hpdflag: StateLib.readPDflag p0 (StateLib.getIndexOfAddr vavalue fstLevel) (memory s) =
  StateLib.readPDflag p0 (StateLib.getIndexOfAddr vavalue fstLevel)
     (add indirection idx
@@ -4710,9 +5600,9 @@ assert(Hpdflag: StateLib.readPDflag p0 (StateLib.getIndexOfAddr vavalue fstLevel
        symmetry.
        apply readPDflagMapMMUPage with entry;trivial.
      rewrite Hpdflag;trivial.
-     cbn. 
+(*      cbn. 
       split;intros;trivial.
-Admitted.
+ *) Admitted.
 
 
 Lemma getPdsVAddrAddIndirection indirection idx   nextIndirection idxroot nbLgen partition part pd entry e w r s vapart:
@@ -4755,6 +5645,9 @@ intros.
       ++ simpl in *.
          destruct Hgoal as [Hgoal|Hgoal];[|apply IHl;trivial].
          subst.
+         assert(Htrue: checkChild partition nbLgen s' vapart = true).
+         rewrite <- Ha.
+         symmetry.
          admit. (** contradiction *)
      * case_eq(checkChild partition nbLgen s' a);intros * Ha1.
       ++ simpl in *.
